proof/security/acai/XMSS_TW.ec
@@ -10,23 +10,11 @@ clone import FL_XMSS_TW as FLXMSSTW.
 require (*--*) DigitalSignatures DigitalSignaturesROM KeyedHashFunctions HashThenSign.
 (*---*) import SA WTW FLXMSSTW_EUFRMA.
 
-
-
-(* --- Parameters --- *)
-(* -- Proof-specific -- *)
-(* Number of allowed signature queries *)
-op qS : { int | 0 <= qS <= l } as rng_qS.
-
-(* Number of allowed random oracle (hash) queries *)
-op qH : { int | 0 <= qH } as ge0_qH.
-
-
-
 (* --- Types --- *)
 (* -- General -- *)
-(* 
-  Seeds (i.e., indexing keys) for PRF that produces (pseudo)randomness 
-  (i.e., indexing keys) for message compression 
+(*
+  Seeds (i.e., indexing keys) for PRF that produces (pseudo)randomness
+  (i.e., indexing keys) for message compression
 *)
 type mseed.
 
@@ -52,7 +40,7 @@ type msgXMSSTW.
 
 clone import FinType as MsgXMSSTW with
   type t <= msgXMSSTW.
-  
+
 (* Signatures *)
 type sigXMSSTW = mkey * sigFLXMSSTW.
 
@@ -64,11 +52,11 @@ clone import FinProdType as MKeyMsgXMSSTW with
   type t2 <- msgXMSSTW,
   theory FT1 <- MKey,
   theory FT2 <- MsgXMSSTW
-  
+
   proof *.
 
 
-    
+
 (* --- Distributions --- *)
 (* Proper distribution over seeds used for PRF that generates (pseudo)randomness for message compression *)
 op [lossless] dmseed : mseed distr.
@@ -79,10 +67,11 @@ op [lossless full uniform] dmkey : mkey distr.
 
 
 (* --- Operators --- *)
-(* PRF that generates indexing keys for message compression given a seed and an index *)  
+(* PRF that generates indexing keys for message compression given a seed and an index *)
 op mkg : mseed -> index -> mkey.
 
 
+abstract theory Original.
 (* -- Proof-specific -- *)
 (* Hash-then-sign proof technique *)
 clone import HashThenSign as HtS with
@@ -94,25 +83,21 @@ clone import HashThenSign as HtS with
   type msg_al_t <= msgXMSSTW,
   type WithPRF.ms_t <= mseed,
   type WithPRF.id_t <= index,
-  
+
     op n <- l,
-    op qS <- qS,
-    op qH <- qH,
-    
+
     op WithPRF.mkg <= mkg,
     op WithPRF.extr_id <= fun (skfl : skFLXMSSTW) => skfl.`1,
-    
+
     op dmsg_fl <= dmsgFLXMSSTW,
     op drco <= dmkey,
     op WithPRF.dms <= dmseed,
-    
+
   theory RCO <= MKey,
   theory MSG_AL <= MsgXMSSTW
-  
+
   proof *.
   realize ge0_n by smt(ge2_l).
-  realize rng_qS by exact: rng_qS.
-  realize ge0_qH by exact: ge0_qH.
   realize dmsg_fl_ll by exact: dmsgFLXMSSTW_ll.
   realize dmsg_fl_uni by exact: dmsgFLXMSSTW_uni.
   realize dmsg_fl_fu by exact: dmsgFLXMSSTW_fu.
@@ -135,16 +120,16 @@ module (XMSS_TW : Scheme_RO) (RO : POracle) = {
     var pk : pkXMSSTW;
     var skfl : skFLXMSSTW;
     var sk : skXMSSTW;
-    
+
     ms <$ dmseed;
-    
+
     (pk, skfl) <@ FL_XMSS_TW.keygen();
-    
+
     sk <- (ms, skfl);
-    
+
     return (pk, sk);
   }
-  
+
   proc sign(sk : skXMSSTW, m : msgXMSSTW) : sigXMSSTW * skXMSSTW = {
     var ms : mseed;
     var skfl : skFLXMSSTW;
@@ -153,99 +138,100 @@ module (XMSS_TW : Scheme_RO) (RO : POracle) = {
     var cm : msgFLXMSSTW;
     var sigfl: sigFLXMSSTW;
     var sig : sigXMSSTW;
-    
+
     ms <- sk.`1;
     skfl <- sk.`2;
-    
+
     idx <- skfl.`1;
-    
+
     mk <- mkg ms idx;
     cm <@ RO.o((mk, m));
-    
+
     (sigfl, skfl) <@ FL_XMSS_TW.sign(skfl, cm);
-    
+
     sig <- (mk, sigfl);
     sk <- (ms, skfl);
-    
+
     return (sig, sk);
   }
-  
+
   proc verify(pk : pkXMSSTW, m : msgXMSSTW, sig : sigXMSSTW) : bool = {
     var mk : mkey;
     var sigfl : sigFLXMSSTW;
     var cm : msgFLXMSSTW;
     var ver : bool;
-    
+
     mk <- sig.`1;
     sigfl <- sig.`2;
-    
+
     cm <@ RO.o((mk, m));
-    
+
     ver <@ FL_XMSS_TW.verify(pk, cm, sigfl);
-     
+
     return ver;
   }
 }.
 
 
 (* --- Reduction adversaries --- *)
+(*
 module (R_PRF_EUFCMAROXMSSTW (A : Adv_EUFCMA_RO) : Adv_PRF) (O : Oracle_PRF) = {
   module O_CMA_R_PRF_EUFCMAROXMSSTW : SOracle_CMA = {
     include var O_Base_Default
-    
+
     var skfl : skFLXMSSTW
-    
+
     proc init(skfl_init : skFLXMSSTW) = {
       skfl <- skfl_init;
       qs <- [];
     }
-    
+
     proc sign(m : msgXMSSTW) : sigXMSSTW = {
       var idx : index;
       var mk : mkey;
       var cm : msgFLXMSSTW;
       var sigfl : sigFLXMSSTW;
       var sig : sigXMSSTW;
-      
+
       idx <- skfl.`1;
-      
+
       mk <@ O.query(idx);
-      
+
       cm <@ MCO.o(mk, m);
-      
+
       (sigfl, skfl) <@ FL_XMSS_TW.sign(skfl, cm);
-      
+
       sig <- (mk, sigfl);
-      
+
       return sig;
     }
   }
-  
+
   proc distinguish() : bool = {
     var pk : pkXMSSTW;
-    var skfl : skFLXMSSTW; 
+    var skfl : skFLXMSSTW;
     var m : msgXMSSTW;
     var sig : sigXMSSTW;
     var is_valid, is_fresh;
-    
+
     MCO.init();
-    
+
     (pk, skfl) <@ FL_XMSS_TW.keygen();
-    
+
     O_CMA_R_PRF_EUFCMAROXMSSTW.init(skfl);
-    
+
     (m, sig) <@ A(MCO, O_CMA_R_PRF_EUFCMAROXMSSTW).forge(pk);
-    
+
     is_valid <@ XMSS_TW(MCO).verify(pk, m, sig);
-    
+
     is_fresh <@ O_CMA_R_PRF_EUFCMAROXMSSTW.fresh(m);
-    
+
     return is_valid /\ is_fresh;
   }
 }.
+*)
 
-
-(* --- Proofs of EUF-CMA property for XMSS-TW (assuming message compression is a RO) --- *) 
+(* --- Proofs of EUF-CMA property for XMSS-TW (assuming message compression is a RO) --- *)
 section Proofs_EUF_CMA_RO_XMSSTW.
 (* -- Declarations -- *)
 (* Models the signing procedure of FL-XMSS-TW *)
@@ -264,17 +250,23 @@ proof. by conseq FLXMSSTW_sign_ll (FLXMSSTW_sign_fun skfl cm). qed.
 declare module A <: Adv_EUFCMA_RO{-FL_XMSS_TW, -ERO, -O_CMA_Default, -O_METCR, -R_EUFCMARO_CRRO, -R_EUFCMARO_METCRRO, -Repro.Wrapped_Oracle, -Repro.RepO, -O_RMA_Default, -R_EUFCMARO_IEUFRMA, -QC_A, -Lazy.LRO, -Repro.ReproGame, -R_EUFRMA_IEUFRMA, -R_PRF_EUFCMARO, -O_PRF_Default, -DSS_AL.DSS.KeyUpdating.O_CMA_Default, -PRF_SK_PRF.O_PRF_Default, -FC.O_THFC_Default, -FC_PRE.O_SMDTPRE_Default, -FC_TCR.O_SMDTTCR_Default, -FC_UD.O_SMDTUD_Default, -O_MEUFGCMA_WOTSTWES, -PKCOC.O_THFC_Default, -PKCOC_TCR.O_SMDTTCR_Default, -TRHC.O_THFC_Default, -TRHC_TCR.O_SMDTTCR_Default, -R_SMDTUDC_Game23WOTSTWES, -R_SMDTTCRC_Game34WOTSTWES, -R_PRF_FLXMSSTWESInlineNOPRF, -R_SMDTPREC_Game4WOTSTWES, -R_MEUFGCMAWOTSTWES_EUFRMAFLXMSSTWESNOPRF, -R_SMDTTCRCTRH_EUFRMAFLXMSSTWESNOPRF, -R_SMDTTCRCPKCO_EUFRMAFLXMSSTWESNOPRF, -R_SMDTTCRCTRH_EUFRMAFLXMSSTWESNOPRF, -R_EUFRMAFLXMSSTW_EUFRMAFLXMSSTWES}.
 
 (* The adversary always terminates if the oracle procedures it can call terminate *)
-declare axiom A_forge_ll (RO <: POracle{-A}) (SO <: SOracle_CMA{-A}) : 
+declare axiom A_forge_ll (RO <: POracle{-A}) (SO <: SOracle_CMA{-A}) :
   islossless RO.o => islossless SO.sign => islossless A(RO, SO).forge.
 
+(* Number of allowed signature queries *)
+declare op qS : { int | 0 <= qS <= l } as rng_qS.
+
+(* Number of allowed random oracle (hash) queries *)
+declare op qH : { int | 0 <= qH } as ge0_qH.
+
 (* The adversary makes a limited number of queries to the given random (hash) oracle and signing oracle *)
-declare axiom A_forge_queries (RO <: POracle{-A, -QC_A}) (SO <: SOracle_CMA{-A, -QC_A}) : 
-  hoare[A(QC_A(A, RO, SO).QC_RO, QC_A(A, RO, SO).QC_SO).forge : 
+declare axiom A_forge_queries (RO <: POracle{-A, -QC_A}) (SO <: SOracle_CMA{-A, -QC_A}) :
+  hoare[A(QC_A(A, RO, SO).QC_RO, QC_A(A, RO, SO).QC_SO).forge :
     QC_A.cH = 0 /\ QC_A.cS = 0 ==> QC_A.cH <= qH /\ QC_A.cS <= qS].
 
 
 (* -- Security theorems -- *)
-(* 
+(*
   High-level security theorem (based on EUF-RMA of FL-XMSS-TW):
   XMSS-TW is EUF-CMA secure in the ROM if mkg (i.e., the function that generates
   indexing keys for the message compression function) is a PRF, MCO (i.e., the message
@@ -282,7 +274,7 @@ declare axiom A_forge_queries (RO <: POracle{-A, -QC_A}) (SO <: SOracle_CMA{-A, 
   secure
 *)
 lemma EUFCMARO_XMSSTW_EUFRMA &m :
-  Pr[EUF_CMA_RO(XMSS_TW, A, O_CMA_Default, MCO).main() @ &m : res]  
+  Pr[EUF_CMA_RO(XMSS_TW, A, O_CMA_Default, MCO).main() @ &m : res]
   <=
   `| Pr[PRF(R_PRF_EUFCMARO(FL_XMSS_TW, A), O_PRF_Default).main(false) @ &m : res] -
      Pr[PRF(R_PRF_EUFCMARO(FL_XMSS_TW, A), O_PRF_Default).main(true) @ &m : res] |
@@ -312,8 +304,8 @@ have ->:
   wp; do 3! rnd.
   while (={w, ERO.m}); 1: by wp; rnd; wp; skip.
   by wp; skip.
-move: (ALKUDSS_EUFCMARO_PRF_CRRO_EUFRMA FL_XMSS_TW FLXMSSTW_sign_ll FLXMSSTW_verify_ll).
-move=> /(_ (fun (skfl : skFLXMSSTW) => skfl.`1 = Index.insubd 0) 
+move: (ALKUDSS_EUFCMARO_PRF_CRRO_EUFRMA FL_XMSS_TW FLXMSSTW_sign_ll FLXMSSTW_verify_ll qS rng_qS qH ge0_qH).
+move=> /(_ (fun (skfl : skFLXMSSTW) => skfl.`1 = Index.insubd 0)
            (fun (skfl : skFLXMSSTW) => (Index.insubd (Index.val skfl.`1 + 1), skfl.`2, skfl.`3, skfl.`4))
            opsign _ FLXMSSTW_sign_fun _ _ _ _).
 + proc; inline *.
@@ -332,19 +324,19 @@ move=> /(_ (fun (skfl : skFLXMSSTW) => skfl.`1 = Index.insubd 0)
   wp; while (true); 1: by wp.
   by wp; skip.
 + move=> i j skfl /= init_sk [ge0i leqS_i] [ge0_j leqS_j] neqj_i.
-  have fupd_it: 
-    forall (k : int), 0 <= k => k < qS => 
-      (fold (fun (sk : skFLXMSSTW) => 
-        ((Index.insubd ((Index.val sk.`1) + 1)), sk.`2, sk.`3, sk.`4)) skfl k).`1 
-      = 
+  have fupd_it:
+    forall (k : int), 0 <= k => k < qS =>
+      (fold (fun (sk : skFLXMSSTW) =>
+        ((Index.insubd ((Index.val sk.`1) + 1)), sk.`2, sk.`3, sk.`4)) skfl k).`1
+      =
       Index.insubd k.
   - elim => [@/fupd | k ge0_k @/fupd ih ltqS_k1].
     * by rewrite fold0.
     rewrite foldS //= ih 2:Index.insubdK //; smt(rng_qS).
   rewrite fupd_it // fupd_it //.
-  move: neqj_i; apply contra => eqins_ij. 
+  move: neqj_i; apply contra => eqins_ij.
   by rewrite -(Index.insubdK i) 2:-(Index.insubdK j) 3:eqins_ij; 1,2: smt(rng_qS).
-+ by sim.  
++ by sim.
 + by sim.
 by move=> /(_ A A_forge_ll A_forge_queries &m).
 qed.
@@ -357,26 +349,26 @@ qed.
   compression function) is a collision-resistant random oracle; prf_sk (i.e., the
   function used to generate WOTS-TW secret keys) is a PRF; f (i.e., the function used
   in the WOTS-TW chains) has SM-DT-UD-C, SM-DT-TCR-C, and SM-DT-PRE-C; pkco (i.e., the
-  fucntion used to compress WOTS-TW public keys to leaves of the binary hash tree) has 
+  fucntion used to compress WOTS-TW public keys to leaves of the binary hash tree) has
   SM-DT-TCR-C; and trh (i.e., the function used to construct the full binary hash tree from
   the leaves) has SM-DT-TCR-C.
 *)
 lemma EUFCMARO_XMSSTW &m :
-  Pr[EUF_CMA_RO(XMSS_TW, A, O_CMA_Default, MCO).main() @ &m : res]  
+  Pr[EUF_CMA_RO(XMSS_TW, A, O_CMA_Default, MCO).main() @ &m : res]
   <=
   `| Pr[MKG_PRF.PRF(R_PRF_EUFCMARO(FL_XMSS_TW, A), O_PRF_Default).main(false) @ &m : res] -
      Pr[MKG_PRF.PRF(R_PRF_EUFCMARO(FL_XMSS_TW, A), O_PRF_Default).main(true) @ &m : res] |
   +
   Pr[CR_RO(R_EUFCMARO_CRRO(FL_XMSS_TW, A), MCO).main() @ &m : res]
   +
-  `|Pr[PRF_SK_PRF.PRF(R_PRF_FLXMSSTWESInlineNOPRF(R_EUFRMAFLXMSSTW_EUFRMAFLXMSSTWES(R_EUFRMA_IEUFRMA(R_EUFCMARO_IEUFRMA(A)))), PRF_SK_PRF.O_PRF_Default).main(false) @ &m : res] - 
+  `|Pr[PRF_SK_PRF.PRF(R_PRF_FLXMSSTWESInlineNOPRF(R_EUFRMAFLXMSSTW_EUFRMAFLXMSSTWES(R_EUFRMA_IEUFRMA(R_EUFCMARO_IEUFRMA(A)))), PRF_SK_PRF.O_PRF_Default).main(false) @ &m : res] -
   Pr[PRF_SK_PRF.PRF(R_PRF_FLXMSSTWESInlineNOPRF(R_EUFRMAFLXMSSTW_EUFRMAFLXMSSTWES(R_EUFRMA_IEUFRMA(R_EUFCMARO_IEUFRMA(A)))), PRF_SK_PRF.O_PRF_Default).main(true) @ &m : res]|
   +
-  (w - 2)%r * 
-`|Pr[FC_UD.SM_DT_UD_C(R_SMDTUDC_Game23WOTSTWES(R_MEUFGCMAWOTSTWES_EUFRMAFLXMSSTWESNOPRF(R_EUFRMAFLXMSSTW_EUFRMAFLXMSSTWES(R_EUFRMA_IEUFRMA(R_EUFCMARO_IEUFRMA(A))))), FC_UD.O_SMDTUD_Default, FC.O_THFC_Default).main(false) @ &m : res] - 
-  Pr[FC_UD.SM_DT_UD_C(R_SMDTUDC_Game23WOTSTWES(R_MEUFGCMAWOTSTWES_EUFRMAFLXMSSTWESNOPRF(R_EUFRMAFLXMSSTW_EUFRMAFLXMSSTWES(R_EUFRMA_IEUFRMA(R_EUFCMARO_IEUFRMA(A))))), FC_UD.O_SMDTUD_Default, FC.O_THFC_Default).main(true) @ &m : res]| 
+  (w - 2)%r *
+`|Pr[FC_UD.SM_DT_UD_C(R_SMDTUDC_Game23WOTSTWES(R_MEUFGCMAWOTSTWES_EUFRMAFLXMSSTWESNOPRF(R_EUFRMAFLXMSSTW_EUFRMAFLXMSSTWES(R_EUFRMA_IEUFRMA(R_EUFCMARO_IEUFRMA(A))))), FC_UD.O_SMDTUD_Default, FC.O_THFC_Default).main(false) @ &m : res] -
+  Pr[FC_UD.SM_DT_UD_C(R_SMDTUDC_Game23WOTSTWES(R_MEUFGCMAWOTSTWES_EUFRMAFLXMSSTWESNOPRF(R_EUFRMAFLXMSSTW_EUFRMAFLXMSSTWES(R_EUFRMA_IEUFRMA(R_EUFCMARO_IEUFRMA(A))))), FC_UD.O_SMDTUD_Default, FC.O_THFC_Default).main(true) @ &m : res]|
   +
-  Pr[FC_TCR.SM_DT_TCR_C(R_SMDTTCRC_Game34WOTSTWES(R_MEUFGCMAWOTSTWES_EUFRMAFLXMSSTWESNOPRF(R_EUFRMAFLXMSSTW_EUFRMAFLXMSSTWES(R_EUFRMA_IEUFRMA(R_EUFCMARO_IEUFRMA(A))))), FC_TCR.O_SMDTTCR_Default, FC.O_THFC_Default).main() @ &m : res] 
+  Pr[FC_TCR.SM_DT_TCR_C(R_SMDTTCRC_Game34WOTSTWES(R_MEUFGCMAWOTSTWES_EUFRMAFLXMSSTWESNOPRF(R_EUFRMAFLXMSSTW_EUFRMAFLXMSSTWES(R_EUFRMA_IEUFRMA(R_EUFCMARO_IEUFRMA(A))))), FC_TCR.O_SMDTTCR_Default, FC.O_THFC_Default).main() @ &m : res]
   +
   Pr[FC_PRE.SM_DT_PRE_C(R_SMDTPREC_Game4WOTSTWES(R_MEUFGCMAWOTSTWES_EUFRMAFLXMSSTWESNOPRF(R_EUFRMAFLXMSSTW_EUFRMAFLXMSSTWES(R_EUFRMA_IEUFRMA(R_EUFCMARO_IEUFRMA(A))))), FC_PRE.O_SMDTPRE_Default, FC.O_THFC_Default).main() @ &m : res]
   +
@@ -395,7 +387,7 @@ have -> /#:
   Pr[EUF_RMA(FL_XMSS_TW, R_EUFRMA_IEUFRMA(R_EUFCMARO_IEUFRMA(A))).main() @ &m : res].
 + by byequiv => //; sim.
 proc; inline *.
-wp; call (: true). 
+wp; call (: true).
 + by move=> RO SO ROll SOll; apply (A_forge_ll RO SO).
 + proc; inline *.
   wp; rnd; skip => />.
@@ -411,3 +403,660 @@ by wp; skip => />; smt(size_eq0 size_ge0).
 qed.
 
 end section Proofs_EUF_CMA_RO_XMSSTW.
+
+end Original.
+
+
+(* Specification closer aligned with the RFC *)
+theory RFC.
+(*---*) import SA.RFC FMap.
+
+type pkXMSSTWRFC = pkFLXMSSTWRFC.
+type skXMSSTWRFC = mseed * skFLXMSSTWRFC.
+(* type msgXMSSTWRFC = msgXMSSTW. *)
+(* type sigXMSSTWRFC = sigXMSSTW. *)
+
+clone import DigitalSignaturesROM as DSS_RFC with
+  type pk_t <- pkXMSSTWRFC,
+  type sk_t <- skXMSSTWRFC,
+  type msg_t <- msgXMSSTW,
+  type sig_t <- sigXMSSTW,
+
+  type in_t <- mkey * (dgstblock * index * msgXMSSTW),
+  type out_t <- msgFLXMSSTW,
+  type d_in_t <- unit,
+  type d_out_t <- bool,
+
+  op doutm <- fun _ => dmsgFLXMSSTW
+proof *.
+
+
+module (XMSS_TW_RFC : DSS_RFC.KeyUpdatingROM.Scheme_RO) (RO : DSS_RFC.RO.POracle) = {
+  proc keygen() : pkXMSSTWRFC * skXMSSTWRFC = {
+    var ms : mseed;
+    var pk : pkXMSSTWRFC;
+    var skfl : skFLXMSSTWRFC;
+    var sk : skXMSSTWRFC;
+
+    ms <$ dmseed;
+    (pk, skfl) <@ FL_XMSS_TW_RFC.keygen();
+    sk <- (ms, skfl);
+
+    return (pk, sk);
+  }
+
+  proc sign(sk : skXMSSTWRFC, m : msgXMSSTW) : sigXMSSTW * skXMSSTWRFC = {
+    var ms : mseed;
+    var skfl : skFLXMSSTWRFC;
+    var idx : index;
+    var root : dgstblock;
+    var mk : mkey;
+    var cm : msgFLXMSSTW;
+    var sigfl : sigFLXMSSTW;
+    var sig : sigXMSSTW;
+
+    ms <- sk.`1;
+    skfl <- sk.`2;
+    idx <- skfl.`1;
+    root <- skfl.`3.`1;
+    mk <- mkg ms idx;
+    (* TODO: cm <@ RO.o((mk, root, idx), m); *)
+    cm <@ RO.o(mk, (root, idx, m));
+    (sigfl, skfl) <@ FL_XMSS_TW_RFC.sign(skfl, cm);
+    sig <- (mk, sigfl);
+    sk <- (ms, skfl);
+
+    return (sig, sk);
+  }
+
+  proc verify(pk : pkXMSSTWRFC, m : msgXMSSTW, sig : sigXMSSTW) : bool = {
+    var mk : mkey;
+    var sigfl : sigFLXMSSTW;
+    var idx : index;
+    var root : dgstblock;
+    var cm : msgFLXMSSTW;
+    var ver : bool;
+
+    root <- pk.`1;
+    mk <- sig.`1;
+    sigfl <- sig.`2;
+    idx <- sigfl.`1;
+    (* TODO: cm <@ RO.o((mk, root, idx), m); *)
+    cm <@ RO.o(mk, (root, idx, m));
+    ver <@ FL_XMSS_TW_RFC.verify(pk, cm, sigfl);
+
+    return ver;
+  }
+}.
+
+clone FinType as IndexFT with
+  type t <= index,
+  op enum <= map Index.insubd (range 0 l)
+
+proof *.
+realize enum_spec.
+move=> x; rewrite count_uniq_mem.
++ rewrite map_inj_in_uniq 2:range_uniq => x0 y0 /mem_range x0in /mem_range y0in eqind.
+  by rewrite -(Index.insubdK _ x0in) -(Index.insubdK _ y0in) eqind.
+rewrite mapP /b2i (: exists (x0 : int), (x0 \in range 0 l) /\ x = Index.insubd x0) 2://.
+by exists (Index.val x); rewrite mem_range Index.valP Index.valKd.
+qed.
+
+clone FinProdType as DBIDX with
+  type t1 <= dgstblock,
+  type t2 <= index,
+
+  theory FT1 <= DigestBlockFT,
+  theory FT2 <= IndexFT
+
+proof *.
+
+clone FinProdType as DBIDXMSGNested with
+  type t1 <= dgstblock * index,
+  type t2 <= msgXMSSTW,
+
+  theory FT1 <= DBIDX,
+  theory FT2 <= MsgXMSSTW
+
+proof *.
+
+clone FinType as DBIDXMSG with
+  type t <= dgstblock * index * msgXMSSTW,
+  op enum <= map (fun (dbim : (_ * _) * _) => (dbim.`1.`1, dbim.`1.`2, dbim.`2)) DBIDXMSGNested.enum
+
+proof *.
+realize enum_spec.
+move => dbim; rewrite count_map /preim.
+by rewrite -(DBIDXMSGNested.enum_spec ((dbim.`1, dbim.`2), dbim.`3)) /#.
+qed.
+
+(* -- Proof-specific -- *)
+(* Hash-then-sign proof technique *)
+clone import HashThenSign as HtSRFC with
+  type pk_fl_t <= pkFLXMSSTWRFC,
+  type sk_fl_t <= skFLXMSSTWRFC,
+  type msg_fl_t <= msgFLXMSSTW,
+  type sig_fl_t <= sigFLXMSSTW,
+  type rco_t <= mkey,
+  type msg_al_t <= dgstblock * index * msgXMSSTW,
+  type WithPRF.ms_t <= mseed,
+  type WithPRF.id_t <= index,
+
+    op n <- l,
+
+    op WithPRF.mkg <= mkg,
+    op WithPRF.extr_id <= fun (skfl : skFLXMSSTWRFC) => skfl.`1,
+
+    op dmsg_fl <= dmsgFLXMSSTW,
+    op drco <= dmkey,
+    op WithPRF.dms <= dmseed,
+
+  theory RCO <= MKey,
+  theory MSG_AL <= DBIDXMSG
+
+  proof *.
+  realize ge0_n by smt(ge2_l).
+  realize dmsg_fl_ll by exact: dmsgFLXMSSTW_ll.
+  realize dmsg_fl_uni by exact: dmsgFLXMSSTW_uni.
+  realize dmsg_fl_fu by exact: dmsgFLXMSSTW_fu.
+  realize drco_ll by exact: dmkey_ll.
+  realize drco_uni by exact: dmkey_uni.
+  realize drco_fu by exact: dmkey_fu.
+  realize WithPRF.dms_ll by exact: dmseed_ll.
+
+import Repro MCORO MCOROLE.
+import EUFRMAEqv DSS_FL DSS_FL_EUFRMA.
+import WithPRF MKG MKG_PRF DSS_AL_PRF KeyUpdatingROM DSS KeyUpdating.
+import WS.
+(*
+module (R_PRF_EUFCMAROXMSSTWRFC (A : Adv_EUFCMA_RO) : Adv_PRF) (O : Oracle_PRF) = {
+  module O_CMA_R_PRF_EUFCMAROXMSSTWRFC : SOracle_CMA = {
+    include var O_Base_Default
+
+    var skfl : skFLXMSSTWRFC
+
+    proc init(skfl_init : skFLXMSSTWRFC) = {
+      skfl <- skfl_init;
+      qs <- [];
+    }
+
+    proc sign(dbim : dgstblock * index * msgXMSSTW) : sigXMSSTW = {
+      var idx : index;
+      var mk : mkey;
+      var cm : msgFLXMSSTW;
+      var sigfl : sigFLXMSSTW;
+      var sig : sigXMSSTW;
+
+      idx <- skfl.`1;
+
+      mk <@ O.query(idx);
+
+      cm <@ MCO.o(mk, dbim);
+
+      (sigfl, skfl) <@ FL_XMSS_TW_RFC.sign(skfl, cm);
+
+      sig <- (mk, sigfl);
+
+      return sig;
+    }
+  }
+
+  proc distinguish() : bool = {
+    var pk : pkXMSSTWRFC;
+    var skfl : skFLXMSSTWRFC;
+    var dbim : dgstblock * index * msgXMSSTW;
+    var sig : sigXMSSTW;
+    var is_valid, is_fresh;
+
+    MCO.init();
+
+    (pk, skfl) <@ FL_XMSS_TW_RFC.keygen();
+
+    O_CMA_R_PRF_EUFCMAROXMSSTWRFC.init(skfl);
+
+    (dbim, sig) <@ A(MCO, O_CMA_R_PRF_EUFCMAROXMSSTWRFC).forge(pk);
+
+    is_valid <@ XMSS_TW_RFC(MCO).verify(pk, dbim.`3, sig);
+
+    is_fresh <@ O_CMA_R_PRF_EUFCMAROXMSSTWRFC.fresh(dbim);
+
+    return is_valid /\ is_fresh;
+  }
+}.
+*)
+
+module (QC_A_RFC (A : DSS_RFC.KeyUpdatingROM.Adv_EUFCMA_RO) : DSS_RFC.KeyUpdatingROM.Adv_EUFCMA_RO)
+                 (RO : DSS_RFC.RO.POracle)
+                 (O : DSS_RFC.DSS.KeyUpdating.SOracle_CMA) = {
+  var cS : int
+  var cH : int
+
+  module QC_SO = {
+    proc sign(m : msgXMSSTW) : sig_al_t = {
+      var sig : sig_al_t;
+
+      cS <- cS + 1;
+      sig <@ O.sign(m);
+
+      return sig;
+    }
+  }
+
+  module QC_RO = {
+    proc o(x : mkey * (dgstblock * index * msgXMSSTW)) : msgFLXMSSTW = {
+      var cm : msgFLXMSSTW;
+
+      cH <- cH + 1;
+      cm <@ RO.o(x);
+
+      return cm;
+    }
+  }
+
+  proc forge(pk : pk_al_t) : msgXMSSTW * sig_al_t = {
+    var m : msgXMSSTW;
+    var sig : sig_al_t;
+
+    cS <- 0;
+    cH <- 0;
+    (m, sig) <@ A(QC_RO, QC_SO).forge(pk);
+
+    return (m, sig);
+  }
+}.
+
+module (R_EUFCMA_EUFCMARFC (A : DSS_RFC.KeyUpdatingROM.Adv_EUFCMA_RO) : Adv_EUFCMA_RO)
+       (RO : RO.POracle) (O : SOracle_CMA) = {
+  var root : dgstblock
+  var idx : index
+
+  module R_O : DSS_RFC.DSS.KeyUpdating.SOracle_CMA = {
+    proc sign(m : msgXMSSTW) : sigXMSSTW = {
+      var sig : sigXMSSTW;
+
+      sig <@ O.sign((root, idx, m));
+
+      idx <- Index.insubd (Index.val idx + 1);
+
+      return sig;
+    }
+  }
+
+  proc forge(pk : pkXMSSTWRFC) : (dgstblock * index * msgXMSSTW) * sigXMSSTW = {
+    var ps : pseed;
+    var m : msgXMSSTW;
+    var sig : sigXMSSTW;
+
+    (root, ps) <- pk;
+    idx <- Index.insubd 0;
+
+    (m, sig) <@ QC_A_RFC(A, RO, R_O).forge(pk);
+
+    return ((root, sig.`2.`1, m), sig);
+  }
+}.
+
+
+(* --- Proofs of EUF-CMA property for XMSS-TW (assuming message compression is a RO) --- *)
+section Proofs_EUF_CMA_RO_XMSSTW.
+(* -- Declarations -- *)
+(* Models the signing procedure of FL-XMSS-TW *)
+declare op opsign : skFLXMSSTWRFC -> msgFLXMSSTW -> sigFLXMSSTW * skFLXMSSTWRFC.
+
+(* opsign precisely captures the semantics of the signing procedure of FL-XMSS-TW *)
+declare axiom FLXMSSTWRFC_sign_fun (skfl : skFLXMSSTWRFC) (cm : msgFLXMSSTW) :
+  hoare[FL_XMSS_TW_RFC.sign: arg = (skfl, cm) ==> res = opsign skfl cm].
+
+(* The signing procedure of FL-XMSS-TW is lossless (and captured by opsign) *)
+local lemma FLXMSSTWRFC_sign_pfun (skfl : skFLXMSSTWRFC) (cm : msgFLXMSSTW) :
+  phoare[FL_XMSS_TW_RFC.sign: arg = (skfl, cm) ==> res = opsign skfl cm] = 1%r.
+proof. by conseq FLXMSSTWRFC_sign_ll (FLXMSSTWRFC_sign_fun skfl cm). qed.
+
+(* Adversary against EUF-CMA in the ROM *)
+declare module A <: DSS_RFC.KeyUpdatingROM.Adv_EUFCMA_RO{
+    -FL_XMSS_TW_RFC, -ERO, -O_CMA_Default, -O_METCR, -R_EUFCMA_EUFCMARFC, -R_EUFCMARO_CRRO,
+    -R_EUFCMARO_METCRRO, -Repro.Wrapped_Oracle, -Repro.RepO, -O_RMA_Default,
+    -R_EUFCMARO_IEUFRMA, -QC_A, -QC_A_RFC, -Lazy.LRO, -Repro.ReproGame, -R_EUFRMA_IEUFRMA,
+    -R_PRF_EUFCMARO, -O_PRF_Default, -DSS_AL.DSS.KeyUpdating.O_CMA_Default,
+    -DSS_RFC.DSS.KeyUpdating.O_CMA_Default,
+    -PRF_SK_PRF.O_PRF_Default, -FC.O_THFC_Default, -FC_PRE.O_SMDTPRE_Default,
+    -FC_TCR.O_SMDTTCR_Default, -FC_UD.O_SMDTUD_Default, -O_MEUFGCMA_WOTSTWES,
+    -PKCOC.O_THFC_Default, -PKCOC_TCR.O_SMDTTCR_Default, -TRHC.O_THFC_Default,
+    -TRHC_TCR.O_SMDTTCR_Default, -R_SMDTUDC_Game23WOTSTWES, -R_SMDTTCRC_Game34WOTSTWES,
+    -R_PRF_FLXMSSTWESInlineNOPRF, -R_SMDTPREC_Game4WOTSTWES, -R_MEUFGCMAWOTSTWES_EUFRMAFLXMSSTWESNOPRF,
+    -R_SMDTTCRCTRH_EUFRMAFLXMSSTWESNOPRF, -R_SMDTTCRCPKCO_EUFRMAFLXMSSTWESNOPRF,
+    -R_SMDTTCRCTRH_EUFRMAFLXMSSTWESNOPRF, -R_EUFRMAFLXMSSTW_EUFRMAFLXMSSTWES}.
+
+(* The adversary always terminates if the oracle procedures it can call terminate *)
+declare axiom A_forge_ll (RO <: DSS_RFC.RO.POracle{-A}) (SO <: DSS_RFC.DSS.KeyUpdating.SOracle_CMA{-A}) :
+  islossless RO.o => islossless SO.sign => islossless A(RO, SO).forge.
+
+local lemma R_forge_ll (RO <: POracle{-R_EUFCMA_EUFCMARFC(A)}) (SO <: SOracle_CMA{-R_EUFCMA_EUFCMARFC(A)}) :
+  islossless RO.o => islossless SO.sign => islossless R_EUFCMA_EUFCMARFC(A, RO, SO).forge.
+proof.
+move => RO_ll SO_ll.
+proc.
+inline 3; wp.
+call (A_forge_ll
+      (<: QC_A_RFC(A, RO, R_EUFCMA_EUFCMARFC(A, RO, SO).R_O).QC_RO)
+      (<: QC_A_RFC(A, RO, R_EUFCMA_EUFCMARFC(A, RO, SO).R_O).QC_SO)) => //.
++ by proc; call RO_ll; wp.
++ by proc; inline 2; wp; call SO_ll; wp.
+by wp.
+qed.
+
+(* Number of allowed signature queries *)
+declare op qS : { int | 0 <= qS <= l } as rng_qS.
+
+(* Number of allowed random oracle (hash) queries *)
+declare op qH : { int | 0 <= qH } as ge0_qH.
+
+(* The adversary makes a limited number of queries to the given random (hash) oracle and signing oracle *)
+declare axiom A_forge_queries (RO <: DSS_RFC.RO.POracle{-A, -QC_A_RFC}) (SO <: DSS_RFC.DSS.KeyUpdating.SOracle_CMA{-A, -QC_A_RFC}) :
+  hoare[A(QC_A_RFC(A, RO, SO).QC_RO, QC_A_RFC(A, RO, SO).QC_SO).forge :
+    QC_A_RFC.cH = 0 /\ QC_A_RFC.cS = 0 ==> QC_A_RFC.cH <= qH /\ QC_A_RFC.cS <= qS].
+
+local lemma R_forge_queries (RO <: POracle{-R_EUFCMA_EUFCMARFC(A), -QC_A})
+                            (SO <: SOracle_CMA{-R_EUFCMA_EUFCMARFC(A), -QC_A}) :
+  hoare[R_EUFCMA_EUFCMARFC(A, QC_A(R_EUFCMA_EUFCMARFC(A), RO, SO).QC_RO, QC_A(R_EUFCMA_EUFCMARFC(A), RO, SO).QC_SO).forge :
+    QC_A.cH = 0 /\ QC_A.cS = 0 ==> QC_A.cH <= qH /\ QC_A.cS <= qS].
+proof.
+proc.
+inline 3; wp; sp.
+call (_:
+      QC_A_RFC.cS = QC_A.cS /\ QC_A_RFC.cH = QC_A.cH
+      /\ QC_A_RFC.cS = 0 /\ QC_A_RFC.cH = 0
+      ==>
+      QC_A.cH <= qH /\ QC_A.cS <= qS) => //.
+conseq (: QC_A_RFC.cS = QC_A.cS /\ QC_A_RFC.cH = QC_A.cH
+         ==>
+         QC_A_RFC.cS = QC_A.cS /\ QC_A_RFC.cH = QC_A.cH)
+       (A_forge_queries
+        (<: QC_A(R_EUFCMA_EUFCMARFC(A), RO, SO).QC_RO)
+        (<: R_EUFCMA_EUFCMARFC(A, QC_A(R_EUFCMA_EUFCMARFC(A), RO, SO).QC_RO, QC_A(R_EUFCMA_EUFCMARFC(A), RO, SO).QC_SO).R_O)) => //.
+proc (QC_A_RFC.cS = QC_A.cS /\ QC_A_RFC.cH = QC_A.cH) => //.
++ proc.
+  inline 2; inline 3.
+  by wp; call (_: true); wp.
+proc.
+inline 2.
+by wp; call (_: true); wp.
+qed.
+(*
+local module R_EUFCMA_EUFCMARFC_QS (RO : RO.POracle) (O : SOracle_CMA) = {
+  include var R_EUFCMA_EUFCMARFC(A, RO, O) [-forge]
+
+  proc forge(pk : pkXMSSTWRFC) : (dgstblock * index * msgXMSSTW) * sigXMSSTW = {
+    var ps : pseed;
+    var m : msgXMSSTW;
+    var sig : sigXMSSTW;
+
+    (root, ps) <- pk;
+    idx <- Index.insubd 0;
+
+    (m, sig) <@ QC_A_RFC(A, RO, R_EUFCMA_EUFCMARFC(A, RO, O).R_O).forge(pk);
+
+    return ((root, sig.`2.`1, m), sig);
+  }
+}.
+
+local lemma EqPr_RQS &m :
+  Pr[EUF_CMA_RO(WithPRF.AL_KU_DSS(FL_XMSS_TW_RFC), R_EUFCMA_EUFCMARFC(A), O_CMA_Default, MCO).main() @ &m : res]
+  =
+  Pr[EUF_CMA_RO(WithPRF.AL_KU_DSS(FL_XMSS_TW_RFC), R_EUFCMA_EUFCMARFC_QS, O_CMA_Default, MCO).main() @ &m : res].
+proof.
+byequiv => //.
+proc.
+inline main; inline{1} 4; inline{2} 4; inline{2} 7.
+seq 7 11: ( ={sig0, pk, m0, R_EUFCMA_EUFCMARFC.root, O_Base_Default.qs, ERO.m}); last by sim.
+wp.
+call (_: ={glob O_CMA_Default, glob R_EUFCMA_EUFCMARFC, ERO.m}).
++ proc.
+  by inline{2} 2; sim.
++ proc.
+  by inline{2} o; wp.
+by conseq />; sim.
+qed.
+
+local lemma R_forge_ll (RO <: POracle{-R_EUFCMA_EUFCMARFC_QS}) (SO <: SOracle_CMA{-R_EUFCMA_EUFCMARFC_QS}) :
+  islossless RO.o => islossless SO.sign => islossless R_EUFCMA_EUFCMARFC_QS(RO, SO).forge.
+proof.
+move=> RO_ll SO_ll.
+proc.
+inline 3; wp; sp.
+call (A_forge_ll
+      (<: QC_A_RFC(A, RO, R_EUFCMA_EUFCMARFC(A, RO, SO).R_O).QC_RO)
+      (<: QC_A_RFC(A, RO, R_EUFCMA_EUFCMARFC(A, RO, SO).R_O).QC_SO)).
++ proc; call RO_ll; by wp.
++ proc; inline 2; wp.
+  by call SO_ll; wp.
+by wp.
+qed.
+
+local lemma R_forge_queries (RO <: POracle{-R_EUFCMA_EUFCMARFC_QS, -QC_A})
+                            (SO <: SOracle_CMA{-R_EUFCMA_EUFCMARFC_QS, -QC_A}) :
+  hoare[R_EUFCMA_EUFCMARFC_QS(QC_A(R_EUFCMA_EUFCMARFC_QS, RO, SO).QC_RO, QC_A(R_EUFCMA_EUFCMARFC_QS, RO, SO).QC_SO).forge :
+    QC_A.cH = 0 /\ QC_A.cS = 0 ==> QC_A.cH <= qH /\ QC_A.cS <= qS].
+proof.
+proc.
+inline 3.
+wp; sp.
+call (_:
+      QC_A_RFC.cS = QC_A.cS /\ QC_A_RFC.cH = QC_A.cH
+      /\ QC_A_RFC.cS = 0 /\ QC_A_RFC.cH = 0
+      ==>
+      QC_A.cH <= qH /\ QC_A.cS <= qS) => //.
+conseq (: QC_A_RFC.cS = QC_A.cS /\ QC_A_RFC.cH = QC_A.cH
+         ==>
+         QC_A_RFC.cS = QC_A.cS /\ QC_A_RFC.cH = QC_A.cH)
+       (A_forge_queries
+        (<: QC_A(R_EUFCMA_EUFCMARFC_QS, RO, SO).QC_RO)
+        (<: R_EUFCMA_EUFCMARFC(A, QC_A(R_EUFCMA_EUFCMARFC_QS, RO, SO).QC_RO, QC_A(R_EUFCMA_EUFCMARFC_QS, RO, SO).QC_SO).R_O)) => //.
+proc (QC_A_RFC.cS = QC_A.cS /\ QC_A_RFC.cH = QC_A.cH) => //.
++ proc.
+  inline 2; inline 3.
+  by wp; call (_: true); wp.
+proc.
+inline 2.
+by wp; call (_: true); wp.
+qed.
+
+*)
+(* local module EUF_CMA_RO_R = { *)
+(*   proc main() : bool = { *)
+(*     var pk : pk_al_t; *)
+(*     var sk : WithPRF.sk_al_t; *)
+(*     var m : dgstblock * index * msgXMSSTW; *)
+(*     var sig : sig_al_t; *)
+(*     var is_valid : bool; *)
+(*     var is_fresh : bool; *)
+
+(*     MCO.init(); *)
+
+(*     (pk, sk) <@ WithPRF.AL_KU_DSS(FL_XMSS_TW_RFC, MCO).keygen(); *)
+(*     DSS_AL_PRF.DSS.KeyUpdating.O_CMA_Default(WithPRF.AL_KU_DSS(FL_XMSS_TW_RFC, MCO)).init(sk); *)
+
+(*     (m, sig) <@ R_EUFCMA_EUFCMARFC(A, MCO, DSS_AL_PRF.DSS.KeyUpdating.O_CMA_Default(WithPRF.AL_KU_DSS(FL_XMSS_TW_RFC, MCO))).forge(pk); *)
+
+(*     is_valid <@ WithPRF.AL_KU_DSS(FL_XMSS_TW_RFC, MCO).verify(pk, m, sig); *)
+(*     is_fresh <@ DSS_AL_PRF.DSS.KeyUpdating.O_CMA_Default(WithPRF.AL_KU_DSS(FL_XMSS_TW_RFC, MCO)).fresh(m); *)
+
+(*     return is_valid /\ is_fresh; *)
+(*   } *)
+(* }. *)
+
+(* -- Security theorems -- *)
+(*
+  High-level security theorem (based on EUF-RMA of FL-XMSS-TW-RFC):
+  XMSS-TW-RFC is EUF-CMA secure in the ROM if mkg (i.e., the function that generates
+  indexing keys for the message compression function) is a PRF, MCO (i.e., the message
+  compression function) is a collision-resistant random oracle, and FL-XMSS-TW-RFC is EUF-RMA
+  secure
+*)
+lemma EUFCMARO_XMSSTWRFC_EUFRMA &m :
+  Pr[DSS_RFC.KeyUpdatingROM.EUF_CMA_RO(XMSS_TW_RFC, A, DSS_RFC.DSS.KeyUpdating.O_CMA_Default, MCO).main() @ &m : res]
+  <=
+  `| Pr[PRF(R_PRF_EUFCMARO(FL_XMSS_TW_RFC, R_EUFCMA_EUFCMARFC(A)), O_PRF_Default).main(false) @ &m : res] -
+     Pr[PRF(R_PRF_EUFCMARO(FL_XMSS_TW_RFC, R_EUFCMA_EUFCMARFC(A)), O_PRF_Default).main(true) @ &m : res] |
+  +
+  Pr[CR_RO(R_EUFCMARO_CRRO(FL_XMSS_TW_RFC, R_EUFCMA_EUFCMARFC(A)), MCO).main() @ &m : res]
+  +
+  Pr[EUF_RMA(FL_XMSS_TW_RFC, R_EUFRMA_IEUFRMA(R_EUFCMARO_IEUFRMA(R_EUFCMA_EUFCMARFC(A)))).main() @ &m : res]
+  +
+  qS%r * (qS + qH + 1)%r * mu1 dmkey witness
+  +
+  l%r * mu1 dmsgFLXMSSTW witness.
+proof.
+have LePrR_A:
+  Pr[DSS_RFC.KeyUpdatingROM.EUF_CMA_RO(XMSS_TW_RFC, A, DSS_RFC.DSS.KeyUpdating.O_CMA_Default, MCO).main() @ &m : res]
+  <=
+  Pr[EUF_CMA_RO(WithPRF.AL_KU_DSS(FL_XMSS_TW_RFC), R_EUFCMA_EUFCMARFC(A), O_CMA_Default, MCO).main() @ &m : res].
++ byequiv => //.
+  proc.
+  inline main.
+  inline fresh verify.
+  inline{2} 4; inline{2} 7.
+  wp; call (: true); 1: by sim.
+  wp; call (: ={ERO.m}); 1: by wp.
+  wp; call (:  ={ERO.m}
+            /\ DSS_RFC.DSS.KeyUpdating.O_CMA_Default.sk{1} = O_CMA_Default.sk{2}
+            /\ DSS_RFC.DSS.KeyUpdating.O_CMA_Default.sk{1}.`2.`3.`1 = R_EUFCMA_EUFCMARFC.root{2}
+            /\ DSS_RFC.DSS.KeyUpdating.O_CMA_Default.sk{1}.`2.`1 = R_EUFCMA_EUFCMARFC.idx{2}
+            /\ (forall m,
+                m \in DSS_RFC.DSS.O_Base_Default.qs{1}
+                <=>
+                m \in map (fun (q : _ * _ * _) => q.`3) O_Base_Default.qs{2})).
+  proc.
+  wp.
+  inline{1} 1.
+  inline{2} 2; inline{2} 3.
+  inline sign.
+  (* wp; call (_: DSS_RFC.DSS.KeyUpdating.O_CMA_Default.sk{1} = O_CMA_Default.sk{2} *)
+  (*           /\ O_CMA_Default.sk{1}.`2.`3.`1 = R_EUFCMA_EUFCMARFC.root{2} *)
+  (*           /\ O_CMA_Default.sk{1}.`2.`1 = Index.insubd R_EUFCMA_EUFCMARFC.idx{2}). *)
+  (* + inline sign. *)
+  (*   wp 19 19. *)
+  wp; call (_: true); 1: by sim.
+  wp; while (={skWOTS0, em, ps0, ad0} /\ sig3{1} = sig5{2}); 1: by sim.
+  wp; call (_: true); 1: by sim.
+  wp; call (_: ={ERO.m}); 1: by wp.
+  wp; skip => &1 &2 /> eqqs _ _ _ mx.
+  rewrite mem_rcons mapP /=; split.
+  + case => [->|].
+    exists ((O_CMA_Default.sk{2}.`2.`3.`1, O_CMA_Default.sk{2}.`2.`1, m{2})); smt(mem_rcons).
+  move=> mxin.
+  move/iffLR: (eqqs mx) => /(_ mxin).
+  rewrite mapP => -[x] [xin /=] eq3.
+  exists x; smt(mem_rcons).
+  move => -[x] []; rewrite mem_rcons /= => -[-> //|].
+  rewrite eqqs mapP => t d; right.
+  exists x => /#.
+  by proc; inline o; wp.
+  seq 1 1 : (={glob A, ERO.m}); 1: by sim.
+  inline init; wp.
+  inline keygen; wp; call (_: true); 1: by sim.
+  auto => &1 &2 /> ms msin ss ssin ps psin sigw /> ->.
+  rewrite /sko2skr /pko2pkr /pkr2pko /= => msig qs1 qs2 sk eqskvl qsrel.
+  rewrite &(contra) qsrel mapP; pose tup := (_, _, _).
+  move=> tp; exists tup => /#.
+move: (ALKUDSS_EUFCMARO_PRF_CRRO_EUFRMA FL_XMSS_TW_RFC FLXMSSTWRFC_sign_ll FLXMSSTWRFC_verify_ll qS rng_qS qH ge0_qH).
+move=> /(_ (fun (skfl : skFLXMSSTWRFC) => skfl.`1 = Index.insubd 0)
+           (fun (skfl : skFLXMSSTWRFC) => (Index.insubd (Index.val skfl.`1 + 1), skfl.`2, skfl.`3))
+           opsign _ FLXMSSTWRFC_sign_fun _ _ _ _).
++ proc; inline *.
+  wp; while (true).
+  - wp; while (true); 1: by wp.
+    wp; while (true); 1: by wp.
+    by wp.
+  by wp; do 2! rnd; skip.
++ move=> skfl.
+  proc; inline *.
+  wp => />; while (true).
+  - wp; while (true); 1: by wp.
+    wp; while (true); 1: by wp.
+    by wp.
+  wp; while (true); 1: by wp.
+  wp; while (true); 1: by wp.
+  by wp; skip.
++ move=> i j skfl /= init_sk [ge0i leqS_i] [ge0_j leqS_j] neqj_i.
+  have fupd_it:
+    forall (k : int), 0 <= k => k < qS =>
+      (fold (fun (sk : skFLXMSSTWRFC) =>
+        ((Index.insubd ((Index.val sk.`1) + 1)), sk.`2, sk.`3)) skfl k).`1
+      =
+      Index.insubd k.
+  - elim => [@/fupd | k ge0_k @/fupd ih ltqS_k1].
+    * by rewrite fold0.
+    rewrite foldS //= ih 2:Index.insubdK //; smt(rng_qS).
+  rewrite fupd_it // fupd_it //.
+  move: neqj_i; apply contra => eqins_ij.
+  by rewrite -(Index.insubdK i) 2:-(Index.insubdK j) 3:eqins_ij; 1,2: smt(rng_qS).
++ by sim.
++ by sim.
+move=> /(_ (R_EUFCMA_EUFCMARFC(A)) R_forge_ll R_forge_queries &m) /#.
+qed.
+
+
+
+(* TODO: Adapt higher-level reductions to consider RFC types *)
+(*
+  Low-level security theorem (based on properties of KHFs and THFs)
+  XMSS-TW is EUF-CMA secure in the ROM if mkg (i.e., the function that generates
+  indexing keys for the message compression function) is a PRF; MCO (i.e., the message
+  compression function) is a collision-resistant random oracle; prf_sk (i.e., the
+  function used to generate WOTS-TW secret keys) is a PRF; f (i.e., the function used
+  in the WOTS-TW chains) has SM-DT-UD-C, SM-DT-TCR-C, and SM-DT-PRE-C; pkco (i.e., the
+  fucntion used to compress WOTS-TW public keys to leaves of the binary hash tree) has
+  SM-DT-TCR-C; and trh (i.e., the function used to construct the full binary hash tree from
+  the leaves) has SM-DT-TCR-C.
+lemma EUFCMARO_XMSSTWRFC &m :
+  Pr[DSS_RFC.KeyUpdatingROM.EUF_CMA_RO(XMSS_TW_RFC, A, DSS_RFC.DSS.KeyUpdating.O_CMA_Default, MCO).main() @ &m : res]
+  <=
+  `| Pr[MKG_PRF.PRF(R_PRF_EUFCMARO(FL_XMSS_TW_RFC, R_EUFCMA_EUFCMARFC(A)), O_PRF_Default).main(false) @ &m : res] -
+     Pr[MKG_PRF.PRF(R_PRF_EUFCMARO(FL_XMSS_TW_RFC, R_EUFCMA_EUFCMARFC(A)), O_PRF_Default).main(true) @ &m : res] |
+  +
+  Pr[CR_RO(R_EUFCMARO_CRRO(FL_XMSS_TW_RFC, R_EUFCMA_EUFCMARFC(A)), MCO).main() @ &m : res]
+  +
+  `|Pr[PRF_SK_PRF.PRF(R_PRF_FLXMSSTWESInlineNOPRF(R_EUFRMAFLXMSSTW_EUFRMAFLXMSSTWES(R_EUFRMA_IEUFRMA(R_EUFCMARO_IEUFRMA(R_EUFCMA_EUFCMARFC(A))))), PRF_SK_PRF.O_PRF_Default).main(false) @ &m : res] -
+  Pr[PRF_SK_PRF.PRF(R_PRF_FLXMSSTWESInlineNOPRF(R_EUFRMAFLXMSSTW_EUFRMAFLXMSSTWES(R_EUFRMA_IEUFRMA(R_EUFCMARO_IEUFRMA(R_EUFCMA_EUFCMARFC(A))))), PRF_SK_PRF.O_PRF_Default).main(true) @ &m : res]|
+  +
+  (w - 2)%r *
+`|Pr[FC_UD.SM_DT_UD_C(R_SMDTUDC_Game23WOTSTWES(R_MEUFGCMAWOTSTWES_EUFRMAFLXMSSTWESNOPRF(R_EUFRMAFLXMSSTW_EUFRMAFLXMSSTWES(R_EUFRMA_IEUFRMA(R_EUFCMARO_IEUFRMA(R_EUFCMA_EUFCMARFC(A)))))), FC_UD.O_SMDTUD_Default, FC.O_THFC_Default).main(false) @ &m : res] -
+  Pr[FC_UD.SM_DT_UD_C(R_SMDTUDC_Game23WOTSTWES(R_MEUFGCMAWOTSTWES_EUFRMAFLXMSSTWESNOPRF(R_EUFRMAFLXMSSTW_EUFRMAFLXMSSTWES(R_EUFRMA_IEUFRMA(R_EUFCMARO_IEUFRMA(R_EUFCMA_EUFCMARFC(A)))))), FC_UD.O_SMDTUD_Default, FC.O_THFC_Default).main(true) @ &m : res]|
+  +
+  Pr[FC_TCR.SM_DT_TCR_C(R_SMDTTCRC_Game34WOTSTWES(R_MEUFGCMAWOTSTWES_EUFRMAFLXMSSTWESNOPRF(R_EUFRMAFLXMSSTW_EUFRMAFLXMSSTWES(R_EUFRMA_IEUFRMA(R_EUFCMARO_IEUFRMA(R_EUFCMA_EUFCMARFC(A)))))), FC_TCR.O_SMDTTCR_Default, FC.O_THFC_Default).main() @ &m : res]
+  +
+  Pr[FC_PRE.SM_DT_PRE_C(R_SMDTPREC_Game4WOTSTWES(R_MEUFGCMAWOTSTWES_EUFRMAFLXMSSTWESNOPRF(R_EUFRMAFLXMSSTW_EUFRMAFLXMSSTWES(R_EUFRMA_IEUFRMA(R_EUFCMARO_IEUFRMA(R_EUFCMA_EUFCMARFC(A)))))), FC_PRE.O_SMDTPRE_Default, FC.O_THFC_Default).main() @ &m : res]
+  +
+  Pr[PKCOC_TCR.SM_DT_TCR_C(R_SMDTTCRCPKCO_EUFRMAFLXMSSTWESNOPRF(R_EUFRMAFLXMSSTW_EUFRMAFLXMSSTWES(R_EUFRMA_IEUFRMA(R_EUFCMARO_IEUFRMA(R_EUFCMA_EUFCMARFC(A))))), PKCOC_TCR.O_SMDTTCR_Default, PKCOC.O_THFC_Default).main() @ &m : res]
+  +
+  Pr[TRHC_TCR.SM_DT_TCR_C(R_SMDTTCRCTRH_EUFRMAFLXMSSTWESNOPRF(R_EUFRMAFLXMSSTW_EUFRMAFLXMSSTWES(R_EUFRMA_IEUFRMA(R_EUFCMARO_IEUFRMA(R_EUFCMA_EUFCMARFC(A))))), TRHC_TCR.O_SMDTTCR_Default, TRHC.O_THFC_Default).main() @ &m : res]
+  +
+  qS%r * (qS + qH + 1)%r * mu1 dmkey witness
+  +
+  l%r * mu1 dmsgFLXMSSTW witness.
+proof.
+move: (EUFRMA_FLXMSSTW (R_EUFRMA_IEUFRMA(R_EUFCMARO_IEUFRMA(A))) _ &m) (EUFCMARO_XMSSTW_EUFRMA &m); last first.
+have -> /#:
+  Pr[FLXMSSTW_EUFRMA.EUF_RMA(FL_XMSS_TW, R_EUFRMA_IEUFRMA(R_EUFCMARO_IEUFRMA(A))).main() @ &m : res]
+  =
+  Pr[EUF_RMA(FL_XMSS_TW, R_EUFRMA_IEUFRMA(R_EUFCMARO_IEUFRMA(A))).main() @ &m : res].
++ by byequiv => //; sim.
+proc; inline *.
+wp; call (: true).
++ by move=> RO SO ROll SOll; apply (A_forge_ll RO SO).
++ proc; inline *.
+  wp; rnd; skip => />.
+  by apply dmkey_ll.
++ proc; inline *.
+  by wp; skip.
+wp; while (true) (size w).
++ move=> z.
+  wp; rnd; wp; skip => /> &1 neqel_w.
+  split; 2: by apply dmsgFLXMSSTW_ll.
+  by elim: (w{1}) neqel_w => //= /#.
+by wp; skip => />; smt(size_eq0 size_ge0).
+qed.
+*)
+end section Proofs_EUF_CMA_RO_XMSSTW.
+end RFC.
