proof/absspec/LTree.ec
@@ -1,0 +1,206 @@
+(* Note: only for reference here, replaced by abstract ltree operator *)
+require import AllCore List RealExp IntDiv Distr DList.
+require (*--*) Subtype.
+
+from Jasmin require import JModel.
+
+require import Params Address Hash WOTS.
+
+(*
+op H_msg_padding_val : W64.t.
+
+op H_msg (t : threen_bytes) (M : W8.t list) : nbytes =
+  let padding : W8.t list = toByte_64 H_msg_padding_val n in
+  Hash (padding ++ ThreeNBytesBytes.val t ++ M).
+*)
+
+subtype wots_keys as WOTSKeys = { l : wots_sk list | size l = 2^h }.
+realize inhabited.
+proof.
+exists (nseq (2^h) witness); rewrite size_nseq; smt(@IntDiv).
+qed.
+
+
+(* 4.1.5 L-Trees *)
+(* takes as input a WOTS+ public key pk and compresses it to a single
+   n-byte value pk[0].
+*)
+
+(*
+  TODO:
+  Is it an issue that the pkco THF will be instantiated with
+  something (ltree) that uses the trh THF (rand_hash)? The
+  SM-DT-TCR-C security model requires the addresses queried to the
+  challenge oracle and the collection oracle to be disjoint.
+  This prevents the adversary doing a collision-like search
+  during the challenge phase by querying the collection oracle.
+  However, if the `pkco` THF internally uses the `trh` THF, then
+  in the SM-DT-TCR-C game for `trh` (where `pkco` is in the collection),
+  the adversary can query the challenge oracle (for `trh) with a certain address,
+  and then query the collection oracle (for `pkco`) with a different address
+  that gets adjusted internally (by `pkco`) to be the same address as the one
+  in the challenge query earlier, right before it calls `trh`. The value returned
+  by the collection oracle might then be a value computed by `trh` using the
+  same address (and public seed) as one of the challenge queries, which is exactly
+  what the disjunctness/disjointness conditions are trying to prevent?
+  Then again, I feel like this might just be abstracted away in the model. Not sure.
+*)
+module LTree = {
+  (* TODO: Replace by abstract THF matching pkco in security spec *)
+  proc ltree (pk : wots_pk, address : adrs, _seed : seed) : nbytes = {
+    var pks : nbytes list;
+    var pk_i : nbytes;
+    var tmp : nbytes;
+    var i : int;
+    var _len : int;
+    var tree_height : int;
+
+    address <- set_tree_height address 0;
+    pks <- LenNBytes.val pk;
+
+    _len <- len;
+    while (1 < _len) { (* Same as _len > 1 *)
+      i <- 0;
+      while (i < _len %/ 2) {
+        address <- set_tree_index address i;
+        pk_i <- nth witness pks (2*i);
+        tmp <- nth witness pks (2*i + 1);
+        pk_i <@ Hash.rand_hash (pk_i, tmp, _seed, address);
+        pks <- put pks i pk_i;
+        i <- i + 1;
+      }
+
+      if (_len %% 2 = 1) {
+        pk_i <- nth witness pks (_len - 1);
+        pks <- put pks (_len %/ 2) pk_i;
+      }
+
+      _len <- if _len %% 2 = 0 then _len %/ 2 else _len %/ 2 + 1;
+
+      tree_height <- get_tree_height address;
+      address <- set_tree_height address (tree_height + 1);
+    }
+
+    pk_i <- nth witness pks 0;
+
+    return pk_i;
+  }
+
+  proc smoosh_level(_seed, _len, address, pks) = {
+    var i, pk_i, tmp, tree_height;
+
+    i <- 0;
+    while (i < _len %/ 2) {
+      address <- set_tree_index address i;
+      pk_i <- nth witness pks (2*i);
+      tmp <- nth witness pks (2*i + 1);
+      pk_i <@ Hash.rand_hash (pk_i, tmp, _seed, address);
+      pks <- put pks i pk_i;
+      i <- i + 1;
+    }
+
+    if (_len %% 2 = 1) {
+      pk_i <- nth witness pks (_len - 1);
+      pks <- put pks (_len %/ 2) pk_i;
+    }
+
+    _len <- if _len %% 2 = 0 then _len %/ 2 else _len %/ 2 + 1;
+
+    tree_height <- get_tree_height address;
+    address <- set_tree_height address (tree_height + 1);
+    return (_len, address, pks);
+  }
+
+  proc smoosh2(_seed, i, address, pks) = {
+    var pk_i, tmp;
+
+    address <- set_tree_index address i;
+    pk_i <- nth witness pks (2*i);
+    tmp <- nth witness pks (2*i + 1);
+    pk_i <@ Hash.rand_hash (pk_i, tmp, _seed, address);
+    pks <- put pks i pk_i;
+    i <- i + 1;
+    return (i, address, pks);
+  }
+}.
+
+op smoosh2 _seed i address (pks : nbytes list) =
+  let address = set_tree_index address i in
+  let pk_i = nth witness pks (2 * i) in
+  let pk_Si = nth witness pks (2 * i + 1) in
+  let pk = rand_hash pk_i pk_Si _seed address in
+  let pks = put pks i pk in
+  (i + 1, address, pks).
+
+hoare smoosh2_eq s0 i0 a0 p0:
+  LTree.smoosh2:
+    _seed = s0 /\ i = i0 /\ address = a0 /\ pks = p0
+    ==> res = smoosh2 s0 i0 a0 p0.
+proof.
+proc; wp.
+ecall (rand_hash_eq pk_i tmp _seed address).
+by auto.
+qed.
+
+op smoosh_level _seed _len address0 pks0 =
+  let (i, address, pks) =
+    fold (fun st=> let (i, address, pks) = st in
+                   smoosh2 _seed i address pks)
+         (0, address0, pks0)
+         (_len %/ 2) in
+  let (len, pks) =
+    if (_len %% 2 = 1)
+    then
+      let pk = nth witness pks (_len - 1) in
+      (_len %/ 2 + 1, put pks (_len %/ 2) pk)
+    else
+      (_len %/ 2, pks)
+  in
+  let tree_height = get_tree_height address in
+  let address = set_tree_height address (tree_height + 1) in
+  (len, address, pks).
+
+hoare smoosh_level_eq s0 l0 a0 p0:
+  LTree.smoosh_level:
+       _seed = s0 /\ _len = l0 /\ address = a0 /\ pks = p0
+    /\ 0 <= _len
+    ==> res = smoosh_level s0 l0 a0 p0.
+proof.
+proc; wp.
+while (   0 <= i /\ i <= _len %/ 2
+       /\ (i, address, pks) = fold (fun st=> let (i, address, pks) = st in smoosh2 _seed i address pks) (0, a0, p0) i).
++ wp; ecall (rand_hash_eq pk_i tmp _seed address).
+  by auto=> /> &0 ge0_i _; rewrite foldS=> /> <- /> /#.
+auto=> /> ge0_l0; rewrite fold0; split.
++ smt().
+move=> address i pks exit ge0_i gei_div2_l0 post.
+have ->> {exit gei_div2_l0}: i = l0 %/ 2 by smt().
+rewrite /smoosh_level -post //=.
+by case: (l0 %% 2 = 1)=> //= /#.
+qed.
+
+op ltree _seed address pk =
+  let address = set_tree_height address 0 in
+  let pks = LenNBytes.val pk in
+  let (_len, address, pks) =
+    fold (fun st=> let (_len, address, pks) = st in
+                   smoosh_level _seed _len address pks)
+         (size pks, address, pks)
+         (ceil (log2 (size pks)%r))
+  in
+  nth witness pks 0.
+
+(* ltree smooshes exactly ceil (log2 len) time; by strong induction on ceil (log2 len):
+   - if len is 1, this is trivial;
+   - if len is 2^n < len <= 2^(n + 1), then the first 2^n nodes smoosh
+     down to a single node in exactly n smooshes (induction, yo); and
+     the remaining len - 2^n smoosh down to a single node in at most n
+     smooshes (induction, yo); then we smoosh those two down with 1
+     more smoosh. (If the rightmost nodes smoosh down to a single node
+     faster than n smooshes, then that node simply gets carried up
+     until the left half is all smooshed down!)
+*)
+hoare ltree_eq s0 a0 pk0:
+  LTree.ltree: pk = pk0 /\ _seed = s0 /\ address = a0 ==> res = ltree s0 a0 pk0.
+proof.
+admitted.
