proof/absspec/Params.ec
@@ -1,0 +1,48 @@
+require import AllCore List RealExp IntDiv.
+require Subtype.
+
+from Jasmin require import JModel.
+
+(* Height of the overall Merkle tree *)
+(* XMSS_TREE_HEIGHT in the implementation *)
+const h : { int | 0 < h } as h_g0.
+
+(* Length of the digest *)
+const n : { int | 1 <= n } as ge1_n.
+
+(* Winternitz parameter: the range of indices into a wots chain *)
+op w : { int | w = 4 \/ w = 16} as w_vals.
+
+const len1 : int = ceil (8%r * n%r / log2 w%r).
+const len2 : int = floor (log2 (len1 * (w - 1))%r / log2 w%r) + 1.
+const len  : int = len1 + len2.
+
+(* TODO: Why are these axioms? *)
+axiom ge0_h : 0 <= h.
+axiom ge0_len  : 0 <= len.
+axiom ge0_len1 : 0 <= len1.
+
+subtype nbytes as NBytes = { l : W8.t list | size l = n}.
+realize inhabited.
+proof.
+by (exists (nseq n W8.zero);smt(size_nseq ge0_n)).
+qed.
+
+subtype len_nbytes as LenNBytes = { l : nbytes list | size l = len }.
+realize inhabited.
+proof.
+by (exists (nseq len witness); smt(size_nseq ge0_len)).
+qed.
+
+subtype onebyte as OneByte = { l : W8.t list | size l = 1 }.
+realize inhabited.
+proof.
+by (exists (nseq 1 witness); smt(size_nseq)).
+qed.
+
+subtype threen_bytes as ThreeNBytesBytes = { l : W8.t list | size l = 3 * n }.
+realize inhabited.
+proof.
+by (exists (nseq (3*n) W8.zero);smt(size_nseq ge0_n)).
+qed.
+
