proof/absspec/Types.ec
@@ -1,0 +1,21 @@
+(* TODO: Mapping between types here and those in security proof (not here, but in proof file) *)
+require import List.
+from Jasmin require import JModel.
+
+require import Params WOTS LTree.
+
+type xmss_sk = { idx : W32.t ;
+                 sk_seed : nbytes ; (* secret *)
+                 sk_prf : nbytes ;
+                 pub_seed_sk : nbytes ; (* public *)
+                 sk_root : nbytes }.
+
+(* Same as single tree variant *)
+type xmss_pk = { pk_oid : W32.t ;
+                 pk_root : nbytes ;
+                 pk_pub_seed : nbytes }.
+
+type msg_t = W8.t list.
+
+
+type xmss_keypair = xmss_sk * xmss_pk.
