proof/absspec/XMSS_Security_RFCAbs.ec
@@ -1,0 +1,90 @@
+require import AllCore IntDiv List StdOrder RealExp Distr DList.
+require import BitEncoding.
+(*---*) import BitChunking.
+
+from Jasmin require import JModel.
+require import Array8.
+
+require (****) XMSS_TW.
+require import XMSS_RFC_Abs.
+import XMSS_RFC_Params Address BaseW.
+
+import IntOrder.
+
+op BitsToBytes (bits : bool list) : W8.t list = map W8.bits2w (chunk W8.size bits).
+op BytesToBits (bytes : W8.t list) : bool list = flatten (map W8.w2bits bytes).
+op W64toBytes_ext (x : W64.t) (l : int) : W8.t list =
+  rev (mkseq (fun i => nth W8.zero (to_list (W8u8.unpack8 x)) i) l).
+
+op idxs2adrs (il : int list) : adrs =
+  init (fun (i : int) =>
+        if 3 <= i <= 6
+        then W32.of_int (nth witness il (6 - i))
+        else W32.zero).
+
+clone XMSS_TW as XMSS_Security with
+  type mseed <- nbytes,
+  type mkey <- nbytes,
+  type msgXMSSTW <- W8.t list,
+  op mkg <-
+    (fun (ms : nbytes) (i : FLXMSSTW.SA.index) =>
+     prf ms (NBytes.insubd (toByte (W32.of_int (FLXMSSTW.SA.Index.val i)) n))),
+  op dmseed <- dmap (dlist W8.dword Params.n) NBytes.insubd,
+  (* TODO: op MKey.enum <- map NBytes.insubd <all W8.t lists of length n>
+  op dmkey <- duniform MKey.enum, *)
+  op FLXMSSTW.n <- n,
+  op FLXMSSTW.log2_w <- ilog 2 w,
+  op FLXMSSTW.h <- h,
+  op FLXMSSTW.chtype <= 0,
+  op FLXMSSTW.pkcotype <= 1,
+  op FLXMSSTW.trhtype <= 2,
+  op FLXMSSTW.SA.dmsgFLXMSSTW <- duniform FLXMSSTW.SA.WTW.DigestBlockFT.enum,
+  type FLXMSSTW.SA.WTW.pseed <- nbytes,
+  type FLXMSSTW.SA.WTW.sseed <- nbytes,
+  op FLXMSSTW.SA.WTW.dsseed <- dmap (dlist W8.dword Params.n) NBytes.insubd,
+  op FLXMSSTW.SA.WTW.dpseed <- dmap (dlist W8.dword Params.n) NBytes.insubd,
+  op FLXMSSTW.SA.WTW.prf_sk <-
+    (fun (ss : nbytes) (psad : nbytes * FLXMSSTW.SA.adrs) =>
+     DigestBlock.insubd (BytesToBits
+                         (NBytes.val
+                          (WOTS.prf_keygen ss (psad.`1, (idxs2adrs (FLXMSSTW.SA.HAX.Adrs.val psad.`2))))))),
+  op FLXMSSTW.SA.WTW.thfc <-
+    (fun (i : int) (ps : nbytes) (ad : FLXMSSTW.SA.adrs) (x : bool list) =>
+     let nb2db = (fun (x : nbytes) => DigestBlock.insubd (BytesToBits (NBytes.val x))) in
+     let mad = (idxs2adrs (FLXMSSTW.SA.HAX.Adrs.val ad)) in
+     if i = 8 * n then
+      nb2db (WOTS.f ps mad (NBytes.insubd (BitsToBytes x)))
+     else if i = 8 * n * 2 then
+      let xl = take (8 * n) x in
+      let xr = drop (8 * n) x in
+      nb2db (rand_hash ps mad (NBytes.insubd (BitsToBytes xl)) (NBytes.insubd (BitsToBytes xl)))
+     else if i = 8 * n * len then
+      let wpk = LenNBytes.insubd (map NBytes.insubd (chunk n (BitsToBytes x))) in
+      nb2db (ltree ps mad wpk)
+     else witness)
+proof *.
+realize FLXMSSTW.ge1_n by exact: ge1_n.
+realize FLXMSSTW.val_log2w by case: w_vals => ->; smt(ilog_powK).
+realize FLXMSSTW.ge1_h by smt(h_g0).
+realize FLXMSSTW.dist_adrstypes by trivial.
+realize FLXMSSTW.SA.WTW.ch0. admitted. (* TODO: instantiate chain *)
+realize FLXMSSTW.SA.WTW.chS. admitted. (* TODO: instantiate chain *)
+realize FLXMSSTW.SA.WTW.two_encodings. admitted. (* TODO: instantiate encoding *)
+realize FLXMSSTW.SA.dmsgFLXMSSTW_ll.
+rewrite duniform_ll -size_eq0 2!size_map size_range.
+suff /#: 0 < 2 ^ (8 * n).
+by rewrite expr_gt0.
+qed.
+realize FLXMSSTW.SA.dmsgFLXMSSTW_uni by exact: duniform_uni.
+realize FLXMSSTW.SA.dmsgFLXMSSTW_fu by apply /duniform_fu /WTW.DigestBlockFT.enumP.
+realize FLXMSSTW.SA.WTW.dsseed_ll by apply /dmap_ll /dlist_ll /W8.dword_ll.
+realize FLXMSSTW.SA.WTW.dpseed_ll by apply /dmap_ll /dlist_ll /W8.dword_ll.
+realize FLXMSSTW.SA.WTW.ddgstblock_ll. admitted. (* TODO: Proof artifact, not needed (might instantiate just because?) *)
+realize MKey.enum_spec. admitted. (* TODO: instantiate enum and prove, but shouldn't be necessary *)
+realize MsgXMSSTW.enum_spec. admitted. (* TODO: this shouldn't be necessary *)
+realize rng_qS. admitted. (* TODO: Proof artifact, move to section *)
+realize ge0_qH. admitted. (* TODO: Proof artifact, move to section *)
+realize dmseed_ll by apply /dmap_ll /dlist_ll /W8.dword_ll.
+realize dmkey_ll. admitted. (* TODO: instantiate and can do *)
+realize dmkey_uni. admitted. (* TODO: instantiate and can do *)
+realize dmkey_fu. admitted. (* TODO: instantiate and can do *)
