proof/absspec/xmss/XMSS_RFC_Abs.ec
@@ -1,0 +1,364 @@
+require import AllCore List IntDiv Distr.
+require (*--*) Subtype.
+
+from Jasmin require import JModel.
+
+require import XMSS_RFC_Params WOTS.
+
+import Address BaseW.
+import Array8.
+
+
+(******************************************************************************)
+(* Types *)
+subtype auth_path as AuthPath = { l : nbytes list | size l = h }.
+realize inhabited.
+proof.
+by exists (nseq h witness); smt(size_nseq ge0_h).
+qed.
+
+type xmss_sk = { idx : W32.t ;
+                 sk_seed : nbytes ; (* secret *)
+                 sk_prf : nbytes ;
+                 pub_seed_sk : nbytes ; (* public *)
+                 sk_root : nbytes }.
+
+type xmss_pk = { pk_oid : W32.t ;
+                 pk_root : nbytes ;
+                 pk_pub_seed : nbytes }.
+
+type xmss_keypair = xmss_sk * xmss_pk.
+
+type sig_t = { sig_idx : W32.t;
+               r : nbytes ;
+               r_sig : (wots_signature * auth_path) }.
+
+type msg_t = W8.t list.
+
+
+(******************************************************************************)
+(* Operators/Oracles *)
+
+(* Corresponds to mkg in security spec *)
+op prf : nbytes -> nbytes -> nbytes.
+
+(* Corresponds to pkco in security spec (modulo lifting input type to bool list) *)
+op ltree : seed -> adrs -> wots_pk -> nbytes.
+
+(* Corresponds to trh in security spec (modulo concatenating two inputs and lifting type to bool list) *)
+op rand_hash : seed -> adrs -> nbytes -> nbytes -> nbytes.
+
+(*
+  Used for message compression oracle, corresponds to mco/MCO in security spec
+  (modulo concatenating public values to output)
+*)
+module type Oracle = {
+  proc o(mkm : threen_bytes * W8.t list) : nbytes
+}.
+
+
+(**********************************************************************************************)
+(* Auxiliary: Treehash/Treesig/RootFromSig *)
+
+(* It is REQUIRED that s % 2^t = 0, i.e., that the leaf at index s is a leftmost leaf of a sub-tree of height t.
+pred leftmost_leaf (s t : int)  = s %% 2^t = 0.
+
+(* Precondition *)
+pred treehash_p (s t : int) = s %% (1 `<<` t) <> 0.
+*)
+
+op nbytes_witness : nbytes = NBytes.insubd (nseq n witness).
+
+
+module TreeHash = {
+  (* Computes the root *)
+  proc treehash(pub_seed sk_seed : seed, s t : int, address : adrs) : nbytes = {
+    var node : nbytes;
+    var stack : nbytes list <- nseq (h  + 1) witness;
+    var heights : W32.t list <- nseq (h + 1) witness; (* Used to manage the height of nodes *)
+    var pk : wots_pk;
+    var offset : W64.t;
+    var i, j : int;
+    var tree_index : W32.t;
+    var node0, node1, new_node : nbytes;
+
+
+    offset <- W64.zero;
+    i <- 0;
+    while (i < 2^t) {
+      address <- set_type address 0;
+      address <- set_ots_addr address (s + i);
+
+      (* Generate the public key from the secret seed *)
+      pk <@ WOTS.pkGen(sk_seed, pub_seed, address);
+
+      address <- set_type address 1;
+      address <- set_ltree_addr address (s + i);
+
+      (* compress the WOTS public key into a single N-byte value *)
+      (* TODO: Replace ltree with THF corresponding to `pkco` in security spec
+      node <@ LTree.ltree(pk, address, pub_seed);
+      *)
+      node <- ltree pub_seed address pk;
+
+      stack <- put stack (to_uint offset) node; (* Push the node onto the stack *)
+      offset <- offset + W64.one;
+      heights <- put heights (to_uint (offset - W64.one)) W32.zero;
+
+      address <- set_type address 2;
+
+      while (
+          (of_int 2)%W64 \ule offset /\ (* The stack needs to have at least two nodes *)
+          nth witness heights (to_uint (offset - W64.one)) =
+             nth witness heights (to_uint (offset - (of_int 2)%W64))
+      ) {
+          tree_index <- W32.of_int(s + i) `>>` truncateu8 (((nth witness heights (to_uint (offset - W64.one))) + W32.one) `&` (of_int 31)%W32);
+
+          address <- set_tree_height address (to_uint (nth witness heights (to_uint (offset - W64.one))));
+          address <- set_tree_index address (W32.to_uint tree_index);
+
+          node0 <- nth nbytes_witness stack (to_uint (offset - W64.of_int 2));
+          node1 <- nth nbytes_witness stack (to_uint (offset - W64.one));
+          (* TODO: Replace rand_hash with THF corresponding to `trh` in security spec
+          new_node <@ Hash.rand_hash(node0, node1, pub_seed, address);
+          *)
+          new_node <- rand_hash pub_seed address node0 node1;
+
+          stack <- put stack (to_uint (offset - W64.of_int 2)) new_node; (* push new node onto the stack *)
+          offset <- offset - W64.one; (* One less node on the stack (removed node0 and node1 and added new_node) *)
+          heights <- put heights
+                   (to_uint (offset - W64.one))
+                   (nth witness heights (to_uint (offset - W64.one)) + W32.one); (* The new node is one level higher than the nodes used to compute it *)
+      }
+
+      i <- i + 1;
+    }
+
+    node <- nth witness stack 0;
+    return node;
+  }
+}.
+
+module TreeSig = {
+  (* Compute the authentication path for the i-th WOTS+ key pair *)
+  proc buildAuthPath(pub_seed sk_seed : seed, idx : W32.t, address : adrs) : auth_path = {
+    var authentication_path : nbytes list;
+    var j : int <- 0;
+    var k : int;
+    var t : nbytes <- witness;
+
+    authentication_path <- nseq h witness;
+
+    while (j < h) {
+      (* k <- floor((W32.to_uint idx)%r / (2^j)%r); XOR ONE *)
+      k <- to_uint ((idx `>>` (of_int j)%W8) `^` W32.one); (* Does this make sense ???? I think so *)
+      t <@ TreeHash.treehash(pub_seed,sk_seed, k * (2^j), j, address);
+      authentication_path <- put authentication_path j t;
+      j <- j + 1;
+    }
+
+    return AuthPath.insubd authentication_path;
+  }
+
+  (*
+   Algorithm 11: treeSig - Generate a WOTS+ signature on a message with
+   corresponding authentication path
+
+     Input: n-byte message M', XMSS private key SK
+            signature index idx_sig, ADRS
+     Output: Concatenation of WOTS+ signature sig_ots and
+             authentication path auth
+  *)
+  proc treesig(M : nbytes, sk : xmss_sk, idx : W32.t, address : adrs) : wots_signature * auth_path  = {
+    var auth : auth_path;
+    var sig_ots : wots_signature;
+    var ots_sk : wots_sk;
+    var sk_seed : nbytes <- sk.`sk_seed;
+    var pub_seed : nbytes <- sk.`pub_seed_sk;
+
+    auth <@ buildAuthPath (pub_seed,sk_seed, idx, address);
+    address <- set_type address 0;
+    address <- set_ots_addr address (W32.to_uint idx);
+
+    sig_ots <@ WOTS.sign_seed(NBytes.val M, sk_seed, pub_seed, address);
+
+    return (sig_ots, auth);
+  }
+}.
+
+(* Compute root from signature *)
+module RootFromSig = {
+  proc rootFromSig(idx_sig : W32.t, sig_ots : wots_signature, auth : auth_path, M : nbytes,
+                   _seed : seed, address : adrs): nbytes = {
+    var pk_ots : wots_pk;
+    var k : int;
+    var nodes0, nodes1 : nbytes;
+    var index : int;
+    var auth_k : nbytes;
+
+    address <- set_type address 0;
+    address <- set_ots_addr address (W32.to_uint idx_sig);
+
+    pk_ots <@ WOTS.pkFromSig(M, sig_ots, _seed, address);
+
+    address <- set_type address 1;
+    address <- set_ltree_addr address (W32.to_uint idx_sig);
+    (* TODO: Replace ltree with THF corresponding to `pkco` in security spec
+    nodes0 <@ LTr.ltree(pk_ots, address, _seed); *)
+    nodes0 <- ltree _seed address pk_ots;
+
+    address <- set_type address 2;
+    address <- set_tree_index address (W32.to_uint idx_sig);
+
+    k <- 0;
+    while (k < h) {
+      address <- set_tree_height address k;
+
+      if (floor ((W32.to_uint idx_sig)%r / (2^k)%r) %% 2 = 0) {
+        index <- get_tree_index address;
+        address <- set_tree_index address (index %/ 2);
+
+        auth_k <- nth witness (AuthPath.val auth) k;
+        (* TODO: Replace rand_hash with THF corresponding to `trh` in security spec
+        nodes1 <@ Hash.rand_hash (nodes0, auth_k, _seed, address);
+        *)
+        nodes1 <- rand_hash _seed address nodes0 auth_k;
+      } else {
+        index <- get_tree_index address;
+        address <- set_tree_index address ((index - 1) %/ 2);
+
+        auth_k <- nth witness (AuthPath.val auth) k;
+        (* TODO: Replace rand_hash with THF corresponding to `trh` in security spec
+        nodes1 <@ Hash.rand_hash (auth_k, nodes0, _seed, address);
+        *)
+        nodes1 <- rand_hash _seed address auth_k nodes0;
+      }
+
+      nodes0 <- nodes1;
+      k <- k + 1;
+    }
+
+    return nodes0;
+  }
+}.
+
+
+
+module XMSS_RFC_Abs (H_msg : Oracle) = {
+  proc sample_randomness () : nbytes * nbytes * nbytes = {
+    var sk_seed, sk_prf, pub_seed : W8.t list;
+
+    sk_seed  <$ DList.dlist W8.dword n;
+    sk_prf   <$ DList.dlist W8.dword n;
+    pub_seed <$ DList.dlist W8.dword n;
+
+    return (NBytes.insubd sk_seed, NBytes.insubd sk_prf, NBytes.insubd pub_seed);
+  }
+
+   proc kg() : xmss_keypair = {
+      var pk : xmss_pk <- witness;
+      var sk : xmss_sk <- witness;
+
+      var sk_seed, sk_prf, pub_seed, root : nbytes;
+
+      var address : adrs <- zero_address;
+      address <- set_layer_addr address 0;
+
+      (sk_seed, sk_prf, pub_seed) <@ sample_randomness();
+
+      sk <- {| idx=W32.zero;
+               sk_seed=sk_seed;
+               sk_prf=sk_prf;
+               pub_seed_sk=pub_seed;
+               sk_root=witness;
+             |};
+
+      root <@ TreeHash.treehash(pub_seed, sk_seed, 0, h, address);
+
+      sk <- {| idx=W32.zero;
+               sk_seed=sk_seed;
+               sk_prf=sk_prf;
+               pub_seed_sk=pub_seed;
+               sk_root=root;
+             |};
+
+      pk <- {| pk_oid=impl_oid; pk_root=root; pk_pub_seed=pub_seed |};
+
+      return (sk, pk);
+  }
+
+  proc sign(sk : xmss_sk, m : msg_t) : sig_t * xmss_sk = {
+    var idx : W32.t;
+    var idx_new : W32.t;
+    var address : adrs;
+    var _R : nbytes;
+    var _M' : nbytes;
+    var ots_sig : wots_signature;
+    var auth : auth_path;
+    var sig : sig_t;
+    var idx_bytes : nbytes;
+    var idx_nbytes : nbytes;
+    var root : nbytes;
+    var t : threen_bytes;
+    var sk_prf : nbytes <- sk.`sk_prf;
+
+    idx <- sk.`idx;
+    idx_new <- sk.`idx + W32.one;
+    sk <- {| sk with idx=idx_new |};
+    address <- zero_address;
+
+    idx_bytes <- NBytes.insubd (toByte idx n);
+
+    (* TODO: Replace with KHF corresponding to mkg in security spec
+    _R <@ Hash.prf(idx_bytes, sk_prf);
+    *)
+    _R <- prf sk_prf idx_bytes;
+
+    root <- sk.`sk_root;
+    t <- ThreeNBytesBytes.insubd (NBytes.val _R ++ NBytes.val root ++ NBytes.val idx_bytes);
+
+    (* TODO: Replace H_msg with relevant RO
+    _M' <- H_msg t m;
+    *)
+    _M' <@ H_msg.o((t, m));
+
+    (ots_sig, auth) <@ TreeSig.treesig(_M', sk, idx, address);
+
+    sig <- {| sig_idx = idx; r = _R ; r_sig = (ots_sig, auth) |};
+
+    return (sig, sk);
+  }
+
+  proc verify(pk : xmss_pk, m : msg_t, s : sig_t) : bool = {
+    var is_valid : bool;
+    var idx_sig : W32.t;
+    var idx_bytes : nbytes;
+    var node, root, _R, _M': nbytes;
+    var auth : auth_path;
+    var sig_ots : wots_signature;
+    var _seed : seed;
+    var address : adrs;
+    var t : threen_bytes;
+
+    idx_sig <- s.`sig_idx;
+    idx_bytes <- NBytes.insubd (toByte idx_sig n);
+    _seed <- pk.`pk_pub_seed;
+    address <- zero_address;
+    (sig_ots,auth) <- s.`r_sig;
+
+    root <- pk.`pk_root;
+    _R <- s.`r;
+    t <- ThreeNBytesBytes.insubd (NBytes.val _R ++ NBytes.val root ++ NBytes.val idx_bytes);
+
+    (* TODO: Replace H_msg with relevant RO
+    _M' <- H_msg t m;
+    *)
+    _M' <@ H_msg.o((t, m));
+
+    node <@ RootFromSig.rootFromSig(idx_sig, sig_ots, auth, _M', _seed, address);
+
+    is_valid <- (node = root);
+
+    return is_valid;
+  }
+}.
