proof/absspec/xmss/XMSS_Types.ec
@@ -1,0 +1,22 @@
+(* TODO: Mapping between types here and in security spec (not here, but in equivalence proof) *)
+require import AllCore List RealExp IntDiv.
+require (*  *) Subtype.
+
+require export XMSS_Params WOTS.
+
+from Jasmin require import JModel.
+
+require import Types Array8 LTree.
+import Params.
+
+subtype auth_path as AuthPath = { l : nbytes list | size l = h }.
+realize inhabited.
+proof.
+by exists (nseq h witness); smt(size_nseq ge0_h).
+qed.
+
+type sig_t = { sig_idx : W32.t;
+               r : nbytes ;
+               r_sig : (wots_signature * auth_path) }.
+
+(******************************************************************************)
