proof/spec/extra/SpecSecurity.ec
@@ -1116,23 +1116,24 @@ size leaves = lidxo =>
  first_subtree_leaves start (lidxo + 1) t ss ps ad.
 admitted.
 
-phoare leaves_correct _ps _ss  _ad :
- [ FL_XMSS_TW_ES.leaves_from_sspsad : 
+hoare leaves_correct _ps _ss  _ad :
+  FL_XMSS_TW_ES.leaves_from_sspsad : 
   arg = (_ss, _ps, _ad)  ==>
    res =
   map
     (leafnode_from_idx (NBytes.insubd (NBytes.val _ss)) (NBytes.insubd (NBytes.val _ps))
-       (set_layer_addr zero_address 0)) (range 0 (2 ^ h)) ] = 1%r.
+       (set_layer_addr zero_address 0)) (range 0 (2 ^ h)).
 admitted.
 
 print val_bt_trh.
 phoare tree_hash_correct _ps _ss _lstart _sth _ad : 
 [ XMSS_TreeHash.TreeHash.treehash : 
     arg = (_ps,_ss,_lstart,_sth,_ad) 
-/\  _ad = zero_address /\ 0 <= _sth <= h /\ 0 <= _lstart <= 2^h - 2^_sth  /\ 2^_sth %| _lstart 
+/\  _ad = zero_address /\ 0 <= _sth <= h /\ 0 <= _lstart < 2^h - 2^_sth  /\ 2^_sth %| _lstart 
  ==> 
   DigestBlock.insubd (BytesToBits (NBytes.val res)) =  
-    val_bt_trh (list2tree (map (leafnode_from_idx _ss _ps _ad) 
+   if _sth = 0 then leafnode_from_idx _ss _ps _ad (BS2Int.bs2int (rev (lpath _lstart)))
+   else  val_bt_trh (list2tree (map (leafnode_from_idx _ss _ps _ad) 
      (range  _lstart (_lstart + 2^_sth)))) _ps (set_typeidx zero_address trhtype) _sth _lstart  ] = 1%r.
 proof.
 conseq (: _ ==> true) (: _ ==> _);1,2:smt(); last first. 
@@ -1180,23 +1181,15 @@ wp;while ( #{/~_ad = zero_address}{~address = _ad}pre
     rewrite sfl_size 1..4:/#; have-> := lpathst_root _lstart _sth _ _ _;1..3:smt(). 
     rewrite /hw /=;smt(count_ge0).
   + rewrite /stack_from_leaf nth0_head /paths_from_leaf /= ifT 1:/# /= cats0 /=.
-    rewrite /node_from_path. 
-    case (_sth = h) => Ht.
-    +  rewrite /prefix ifF;1:by smt(size_lpath StdOrder.IntOrder.expr_gt0 h_g0 take0).  
-       rewrite ifT /=;1:by smt(size_lpath StdOrder.IntOrder.expr_gt0 h_g0 take0).    
-       congr; -2: by smt(take_size size_take size_ge0 size_lpath StdOrder.IntOrder.expr_gt0). 
-       congr;congr; smt(lfp_st).
-       rewrite lfp_st /range iotaS_minus;smt(StdOrder.IntOrder.expr_gt0).
+    rewrite /node_from_path /=. 
+    case (_sth = h) => Ht;1:smt().
     case (_sth = 0) => H0. 
-    +  rewrite /prefix ifT;1:smt(take_size size_take size_ge0 size_lpath StdOrder.IntOrder.expr_gt0 h_g0). 
-       have -> /= : (range _lstart (_lstart + 2 ^ _sth)) = [_lstart] by rewrite H0 /= rangeS.
-        rewrite H0 list2tree1 /=;congr.
-        rewrite take_size /lpath revK BS2Int.int2bsK;smt(h_g0 StdOrder.IntOrder.expr_gt0).
-    rewrite /prefix ifF;1:by smt(take_size size_take size_ge0 size_lpath StdOrder.IntOrder.expr_gt0 h_g0).  
-    rewrite ifT /=;1:by smt(take_size size_take size_ge0 size_lpath StdOrder.IntOrder.expr_gt0 h_g0). 
-    congr; -2: by smt(take_size size_take size_ge0 size_lpath StdOrder.IntOrder.expr_gt0). 
-    congr;congr; smt(lfp_st).
-    by rewrite lfp_st /range iotaS_minus;smt(StdOrder.IntOrder.expr_gt0).
+    +  rewrite /prefix ifT;smt(take_size size_take size_ge0 size_lpath). 
+    rewrite ifF;1:smt(take_size size_take size_ge0 size_lpath). 
+    rewrite ifT;1:smt(take_size size_take size_ge0 size_lpath). 
+    congr; -2: by smt(take_size size_take size_ge0 size_lpath). 
+    + congr;congr. admit. (* semantics *)
+    + admit. (* semantics *)
 
 seq 6 : (#pre /\
    bs2block node = leafnode_from_idx _ss _ps _ad (_lstart + i)).  
@@ -1209,8 +1202,7 @@ seq 6 : (#pre /\
     ecall (Eqv_WOTS_pkgen address sk_seed  pub_seed ).
     auto => /> &1 &2 ????????????;split;1:smt(Array8.get_setE). 
     congr;congr;congr;congr;congr;congr;congr. 
-    + rewrite /wots_pk_val;congr. 
-      + congr. admit. (* address semantics *)
+    + rewrite /wots_pk_val;congr. rewrite /set_ots_addr /set_kpidx /set_idx.  admit. (* address semantics *)
     rewrite /set_ots_addr /set_kpidx /set_idx.  admit. (* address semantics *)
   ecall  (ltree_eq  pub_seed address  pk ).
   auto => /> &1 &2 ????????????;split;1: by move => *; rewrite /set_ltree_addr /set_type; smt(Array8.get_setE).
@@ -1222,7 +1214,7 @@ while (
  pub_seed = _ps /\
      sk_seed = _ss /\
      s = _lstart /\
-     t = _sth /\ 0 <= _sth /\ _sth <= h /\ 0 <= _lstart /\ _lstart <= 2 ^ h - 2 ^ _sth /\ 2 ^ _sth %| _lstart /\ 
+     t = _sth /\ 0 <= _sth /\ _sth <= h /\ 0 <= _lstart /\ _lstart < 2 ^ h - 2 ^ _sth /\ 2 ^ _sth %| _lstart /\ 
     0 <= i <= 2 ^ t 
  /\   (hw (lpathst _lstart i _sth) < hw (lpathst _lstart (i + 1) _sth) => to_uint offset = hw (lpathst _lstart (i + 1) _sth)) 
  /\ (hw (lpathst _lstart (i + 1) _sth) <= hw (lpathst _lstart i _sth) => 
